\documentclass[../hw3]{subfiles}
\begin{document}
\begin{problem}
$\forall x \not\in \Z\setminus \{0\}$, let $f(x)=2x \sum_{1}^{\infty} \frac{1}{x^2-n^2}$.
Show $f\in C^1$ on the given domain and \[
	f'(x)=-\sum_{1}^{\infty} \left[ \frac{1}{(x-n)^2}+\frac{1}{(x+n)^2} \right]
	.\]
\end{problem}
\begin{proof}
	We have that, for $x \neq n \in \Z\setminus \{0\}$, \[
		f_n'(x)=\frac{2(x^2 - n^2) - 4x^2}{(x^2 - n^2)^2}=\frac{-2(x^2  + n^2)}{(x^2 - n^2)^2}=-\frac{(x-n)^2 + (x+n)^2}{((x-n)(x+n))^2}=-\left( \frac{1}{(x-n)^2} + \frac{1}{(x+n)^2} \right)
		.\]

	So, $f_n \in  C^1$ on such a domain.

	We have seen that $\sum_{1}^{\infty} \frac{1}{x^2 - n^2}$ will converge on this domain in Problem 4.

	So, $2x \sum_{1}^{\infty} \frac{1}{x^2 - n^2}$ will converge as well.

	We now wish to show that  $f_n'(x)$ converges uniformly to $-\left( \frac{1}{(x-n)^2} + \frac{1}{(x+n)^2} \right)$.

	Consider $x \in [k+\epsilon, k+1-\epsilon],\,  \forall 0<\epsilon<\frac{1}{2}, \forall k\in \Z\setminus \{0\}$ as in Problem 4.

	Then, we will construct a bounding sequence $|f_n|\le M_n,\,  \forall n$ such that $\sum M_n$ converges.

	Since $x \in [k+\epsilon, k+1-\epsilon]$, we have $|x|\le \epsilon < 1$.

	So, $|x \pm n| \ge n - |x| > n - 1$. Then, $(x \pm n)^2 > (n-1)^2$.

	Thus, $\left|\frac{1}{(x + n)^2} + \frac{1}{(x-n)^2}\right| < \frac{2}{(n-1)^2}\approx 1 / n^2$.

	Since $\sum M_n = \sum \frac{2}{(n-1)^2}$ converges by comparison to $\sum n^{-2}$, then $f_n'(x)$ converges uniformly by Weierstrass.

	Thus, by Theorem 7.13, we have that \[
		f'(x)=-\sum_{1}^{\infty} \left[ \frac{1}{(x-n)^2}+\frac{1}{(x+n)^2} \right]
		,\] which is what we wanted to prove.
\end{proof}
\end{document}
