\documentclass[../hw8]{subfiles}

\begin{document}

\subsection*{72}
Prove the proposition.

\begin{proposition}
    For all $x>0$ and $n\in\mathbb{Z}^+$,
    \[e^x>1+x+\frac{x^2}{2!}+\frac{x^3}{3!}+\cdots+\frac{x^n}{n^!}=\sum\limits_{k=0}^{n}\frac{x^k}{k!}.\]
\end{proposition}

\begin{proof}
    Since $e^x>1$ for all $x>0$, then, by 5.8.4, \[\int e^t\,dt > \int dt.\]

    So, \[1+\int_{0}^{x}e^t\,dt >1+\int_{0}^{x} dt.\]

    But \[e^x=1+\int_{0}^{x}e^t\,dt >1+\int_{0}^{x} dt=1+x,\]

    So \[e^x>1+x.\]

    Then, \[1+\int_{0}^{x}e^t\,dt >1+\int_{0}^{x} 1+t dt.\]

    So, \[e^x>1+x+\frac{x^2}{2}.\]

    If we continue on in this manner, after $n$ times we will achieve
    \[e^x>1+x+\frac{x^2}{2}+\cdots+\frac{x^n}{n!}=\sum\limits_{k=0}^{n}\frac{x^k}{k!}.\]

    So,
    \begin{align*}
        1+\int_{0}^{x}&>1+\int_{0}^{x}\sum\limits_{k=0}^{n}\frac{t^k}{k!}\,dt \\
        e^x&>\sum\limits_{k=0}^{n} \int_{0}^{x} \frac{t^k}{k!}\,dt, \quad \text{by 5.4.4, linearity of the integral} \\
        e^x&>\sum\limits_{k=0}^{n} \frac{t^{k+1}}{(k+1)!} \\
        e^x&>\sum\limits_{k=0}^{n+1}\frac{x^k}{k!}. \\
    \end{align*}

    So, we have shown that $e^x>\sum\limits_{k=0}^{n}\frac{x^k}{k!}$ for $n=1$, where $e^x>1+x$, for $n$, which covers the inductive hypothesis, and finally for $n+1$.

    Therefore, by induction, the proposition holds.



    % Since $\int_{0}^{x}e^t\,dt = e^x-1$, then $e^x=1+\int_{0}^{x}e^t\,dt$.

    % We will prove by induction on $n$ that, 
    % \[e^x-1=\int_{0}^{x}e^t\,dt>\int_{0}^{x}\sum\limits_{k=0}^{n-1}\frac{t^k}{k!}\,dt.\]

    % For the base case, when $n=1$, 
    % \begin{align*}
    %     e^x-1=\int_{0}^{x}e^t\,dt&>\int_{0}^{x}\sum_{k=0}^{0}\frac{t^k}{k!}\,dt=\int_{0}^{x}dt=x\\
    %     e^x&>1+x,
    % \end{align*}

    % which is true for $x>0$, so the base case holds.
    

    % % Since $e^x$ is increasing, and $e^0=1$, then $e^x>1$ for all $x>0$.

    % % Since $\frac{d}{dx}[e^x]=e^x>1=\frac{d}{dx}[1+x]$ for all $x>0$, then $e^x$ is increasing faster than $x+1$ for all $x>0$.

    % % Since, at $x=0$, $e^0=0+1$, then $e^x>1+x$ for all $x>0$.

    % % So, $e^x-1>x$ for all $x>0$, and the base case holds.

    % Assume that $n=m$ holds by the inductive hypothesis,
    % \[\int_{0}^{x}e^t\,dt>\int_{0}^{x}\sum\limits_{k=0}^{m-1}\frac{t^k}{k!}\,dt.\]

    % For the inductive step, we let $n=m+1$,
    % \begin{align*}
    %     \int_{0}^{x}e^t\,dt &> \int_{0}^{x}\sum\limits_{k=0}^{m}\frac{t^k}{k!}\,dt \\
    %     &= \sum_{k=0}^{m} \int_{0}^{x} \frac{t^k}{k!}\,dt \quad \text{(by 5.4.4, linearity of the integral)} \\
    %     &= \sum_{k=0}^{m} {\left[ \frac{t^{k+1}}{(k+1)k!} \right]}_{0}^{x} \\
    %     &= \sum_{k=0}^{m} \frac{x^{k+1}}{(k+1)!} \\
    % \end{align*}

    % Then, we re-index the sum by setting $k$ to $k-1$.

    % So, \[\int_{0}^{x}e^t\,dt = e^x-1 > \sum\limits_{k=1}^{m}\frac{x^k}{k!}.\]

    % But the zeroth term of the sum, at $k=0$, is $\frac{k^0}{0!}=1$. 

    % So, \[1+\sum\limits_{k=1}^{m}\frac{x^k}{k!} = \sum\limits_{k=0}^{m}\frac{x^k}{k!}.\]

    % Then, \[e^x > \sum\limits_{k=0}^{m}\frac{x^k}{k!}.\]

    % Therefore the $n=m+1$ case holds. 

    % Thus, by induction, the proposition holds.
\end{proof}


\subsection*{73}
Prove the proposition.

\begin{proposition}
    If $n$ is a positive integer, then for all $x$ sufficiently large, \[e^x>x^n.\]
\end{proposition}

\begin{proof}
    From 72, we note that, \[e^x>\sum\limits_{k=0}^{n}\frac{x^k}{k!}.\]

    We will show that \[\sum\limits_{k=0}^{n}\frac{x^k}{k!}>x^n.\]
    
    Since the proposition concerns only large $x$, then with $x>0$, 
    \[\sum\limits_{k=0}^{n}\frac{x^k}{k!}>0.\] 

    So, omitting all but the ${n+1}^{\text{th}}$ term of the sum, \[e^x>\frac{x^{n+1}}{(n+1)!},\]
    which we claim is also $\frac{x^{n+1}}{(n+1)!}>x^n$ for sufficiently large $x$.

    Then, with $x>0$ and thus $x^n>0$,
    \begin{align*}
        \frac{x^{n+1}}{(n+1)!} &> x^n \\
        \frac{x}{(n+1)!} &> 1 \\
        x &> (n+1)!.
    \end{align*}

    So, for all $x>{(n+1)!}$, $x$ is sufficiently large such that, 
    \[e^x>x^n.\]


\end{proof}

\end{document}