\documentclass{article}
\begin{document}
  \begin{problem}
    Let $g:\R^{2}\longmapsto\R$ be the function defined by  \[
    g(x,y)=\begin{cases}
      \frac{xy(x^2-y^2)}{x^2+y^2}& \quad (x,y)\neq(0,0),\\
      0& (x,y)=(0,0).\\
    \end{cases}
    \] 
    Show that \[
      g_y(x,0)=\lim\limits_{h\to 0}\frac{g(x,h)-g(x,0)}{h}=x
    \] 
    and similarly that $g_x(0,y)=-y$. Hence, show that $g_{yx}(0,0)=1$ and $g_{xy}(0,0)=-1$.
  \end{problem}

  First, we compute $g_y$ with differentiation and evaluate at $y=0$,
  \begin{align*}
    g_y(x,y) &= \frac{\partial}{\partial y}\left[ \frac{xy(x^2-y^2)}{x^2+y^2} \right] \\ 
             &= \frac{\left[ x(x^2-y^2) \right](x^2+y^2)-\left[ xy(x^2-y^2) \right](2y)}{{(x^2+y^2)}^2} \\
    g_y(x,0) &= \frac{x^5}{x^4} \\
             &= x.
  \end{align*}

  We then compute $g_y$ using the limit definition at $y=0$,
  \begin{align*}
    \lim\limits_{h\to 0}\frac{g(x,h)-g(x,0)}{h} &= \lim\limits_{h\to 0}\frac{\frac{xh(x^2-h^2)}{x^2+h^2}-\frac{x(0)(x^2-0^2)}{x^2+0^2}}{h} \\
                                                &= \lim\limits_{h\to 0}\frac{\frac{xh(x^2-h^2)}{x^2+h^2}}{h} \\
                                                &= \lim\limits_{h\to 0}\frac{x(x^2-h^2)}{x^2+h^2} \\
                                                &= \frac{x^3}{x^2} \\
                                                &= x. \\
  \end{align*}

  So, $g_y(x,0)=x$ by both the limit definition and the derivative computation. For simplicity, we will use the latter method of finding the partials of  $g$. 

  For  $g_x(0,y)$,
  \begin{align*}
    g_x(x,y)&=\frac{[y(x^2-y^2)+2x^2 y](x^2+y^2)-(xy(x^2-y^2))[2x]}{{(x^2+y^2)}^2} \\
    g_x(0,y) &= \frac{y(-y^2)y^2}{y^4} \\
             &= -y. \\
  \end{align*}

  Then, for $g_{yx}(0,0)$, we take the derivative of $g_y(x,0)$ in $x$, $\frac{d}{dx}x=1$. 

  For $g_{xy}(0,0)$, similarly, we take the derivative of $g_x(0,y)$ in  $y$,  $\frac{d}{dx}-y=-1$. 
\end{document}
