\documentclass[../hw4]{subfiles}

\begin{document}

Prove by induction that \[\frac{1}{{(1-x)}^{k+1}}=\sum_{n=0}^{\infty}\binom{n+k}{k}x^n, \quad \forall|x|<1.\] 

\begin{proof}

First, with given by the identity, \[\binom{n}{k}=\frac{n!}{k!(n-k)!},\]
we simplify the binomial coefficient to \[\binom{n+k}{k}=\frac{(n+k)!}{k!n!}.\]

We will rewrite the relationship we wish to demonstrate given the above; we will also move the $k!$ term from the denominator of the sum to the left as it does not depend on the summation index $n$ and reindex the sum starting at $n=1$. 
\[\frac{k!}{{(1-x)}^{k+1}}=1+\sum_{n=1}^{\infty}\frac{(n+k)!}{n!}x^n, \quad \forall|x|<1.\]

We will perform induction on $k\geq0$. We start with the base case $k=0$.
\begin{align*}
    \frac{0!}{{(1-x)}^{0+1}}&=1+\sum_{n=1}^{\infty}\frac{(n+0)!}{n!}x^n \\
    \frac{1}{1-x}&=1+\sum_{n=1}^{\infty}x^n=\sum_{k=0}^{\infty}x^n. \\
\end{align*}

We recognize this equality to hold as the identity of the geometric series. So, the base case holds as well.

We claim that the $k^{\text{th}}$ case holds by the inductive hypothesis,
\[\frac{k!}{{(1-x)}^{k+1}}=1+\sum_{n=1}^{\infty}\frac{(n+k)!}{n!}x^n, \quad \forall|x|<1.\]

Then, for the inductive step, we differentiate the relationship given by the inductive hypothesis. 
\begin{align*}
    \frac{d}{dx}\left[ \frac{k!}{{(1-x)}^{k+1}} \right] &= \frac{d}{dx}\left[1+\sum_{n=1}^{\infty}\frac{(n+k)!}{n!}x^n\right] \\
    \frac{(k+1)!}{{(1-x)}^{k+2}}&=\sum_{n=1}^{\infty}\frac{(n+k)!}{n!}nx^{n-1} \\
    \frac{(k+1)!}{{(1-x)}^{(k+1)+1}}&= \sum_{n=1}^{\infty} \frac{(n-k)!}{(n-1)!}x^{n-1} \\
    &= \sum_{j=0}^{\infty} \frac{(j+1+k)!}{(j+1-1)!}x^{j+1-1} \\
    &= \sum_{j=0}^{\infty} \frac{(j+(k+1))!}{j!}x^j \\
    &= 1 + \sum_{j=1}^{\infty} \frac{(j+(k+1))!}{j!}x^j, \\
\end{align*}

which is the same as the formula with an index of $k+1$. So, by induction, the statement holds.
    
\end{proof}

\end{document}