\documentclass[../hw2]{subfiles}
\begin{document}
\begin{problem}[5]
Let $f:\R\longrightarrow\R$ be continuous. Suppose ${(x_n)}_{n=1}^{\infty}$   converges to $x$.

Prove \[
	\lim\limits_{n\to \infty}\frac{f(x_1)+\cdots+f(x_{n})}{n}=f(x)
	.\]
\end{problem}
\begin{proof}
	Since $(x_n)$ converges to  $x$,  $\forall \epsilon >0,\ \exists N,\ \forall n\ge N,\ |x_n-x|<\epsilon$.

	So, we will split the limit into two parts, where $f$ maps on  $x_n$ which are  $\epsilon$ close to  $x$, and on  $x_n$ which are far from $x$. \[
		\lim_{n\to \infty}\left[ \sum\limits_{i=1}^{N-1}\frac{f(x_i)}{n}+\sum\limits_{i=N}^{n}\frac{f(x_i)}{n} \right] = f(x)
		.\]
	But, the left sum is a finite value by $n$ which exceeds any number, so this quantity will become to zero. Then, since the $x_i$ for $i\ge N$ approach $x$,  $f(x_i)$ will approach  $f(x)$ by sequential continuity. So,
	\begin{align*}
		f(x) & = \lim_{n\to \infty}\sum\limits_{i=N}^{n}\frac{f(x_i)}{n} \\
		     & = \lim_{n\to \infty}\sum\limits_{i=N}^{n}\frac{f(x)}{n}   \\
		     & = \lim_{n\to \infty}\left(\frac{n-N}{n}\right)f(x)        \\
		     & = \lim_{n \to \infty} \left( 1-\frac{N}{n} \right) f(x)   \\
		     & = f(x)
		.\end{align*}
\end{proof}
\end{document}
