\documentclass[../hw5]{subfiles}

\begin{document}

Solve the differential equations and check the solution.
\begin{enumerate}[label= (\alph*)]
    \item $y'=x-4xy$
    
    We begin by reorganizing the equation to the form $y'+p(x)y=q(x)$ in order to arrive at the solution via the method of integrating factors. S.H.E. 9.1.2 Provides that, with $H(x)=\int p(x)\,dx$,
    \[y(x)=e^{-H(x)}\left[ \int e^{H(x)}q(x)\,dx \right],\] with a constant of integration after the evaluation of the indefinate integral.

    So, $y'+4xy=x$ gives \[H(x)=\int 4x\,dx=2x^2.\]

    Then,
    \begin{align*}
        y(x)&=e^{-2x^2}\left[ \int xe^{2x^2}\,dx \right] \\
        &=e^{-2x^2}\left[ \frac{1}{4}\int e^u\,du \right] \\
        &=e^{-2x^2}\left( \frac{e^{2x^2}}{4}+c \right) \\
        &=ce^{-2x^2}+\frac{1}{4}. \\
    \end{align*}

    
    We verify this result by taking the derivative of our solution, 
    \[y'=\frac{d}{dx}\left[ ce^{-2x^2}+\frac{1}{4} \right]=-4cxe^{-2x^2},\]
    and then matching it with the equation for $y$ above,
    \begin{align*}
        y'&=x-4xy\\
        -4cxe^{-2x^2}&=x-4x\left( ce^{-2x^2}+\frac{1}{4} \right) \\
        &=x-4cxe^{-2x^2}-\frac{4x}{4} \\
        &=-4cxe^{-2x^2}. \\
    \end{align*}

    This statement is true, and therefore we have arrived at a valid general solution.

    \item $y'=\csc{x}+y\cot{x}$
    
    Again, we will put the first order linear differential equaition into standard form such that we can use the form provided by S.H.E. 9.1.2.

    With $y'-y\cot{x}=\csc{x}$, we will need $H(x)=\int-\cot{x}\,dx=-\ln{\sin{x}}$.

    Then,
    \begin{align*}
        y(x)&=e^{\ln{\sin{x}}}\left[ \int \csc{x}e^{-\ln{\sin{x}}}\,dx \right] \\
        &=\sin{x}\left[ \int-\frac{dx}{\sin{x}e^{\ln{\sin{x}}}} \right] \\
        &=\sin{x}\left[ \int-\csc^2{x}\,dx \right] \\
        &=\sin{x}\left( -\cot{x}+c \right) \\
        &=c\sin{x}-\cos{x}. \\
    \end{align*}

    We diffentiate our solution,
    \[y'(x)=c\cos{x}+\sin{x}.\]

    We compare this to the given form for $y'(x)$,
    \begin{align*}
        y'(x)&=\csc{x}+y\cot{x}\\
        c\cos{x}+\sin{x}&=\csc{x}+(c\sin{x}-\cos{x})\cot{x}\\
        &=\frac{1}{\sin{x}}+c\cos{x}-\frac{\cos^2{x}}{\sin{x}}\\
        &=\frac{1-\cos^2{x}}{\sin{x}}+c\cos{x}\\
        &=\frac{\sin^2{x}}{\sin{x}}+c\cos{x} \\
        &=\sin{x}+c\cos{x}. \\
    \end{align*}

    We see that the statement is true and so the general solution is valid.

    \item $x^2y'+2xy=8x^3$
    
    We put this equation into standard form and proceed with the methods used in the previous problems,
    \[y'+\frac{2}{x}y=8x.\]

    With, $\int p(x)\,dx=\int\frac{2}{x}\,dx=2\ln{x}$,
    \begin{align*}
        y(x)&=e^{-2\ln{x}}\left[ \int 8xe^{2\ln{x}}\,dx \right] \\
        &=\frac{1}{x^2}\left[ \int 8x^3\,dx \right] \\
        &=\frac{1}{x^2}\left( 2x^4+c \right) \\
        &=2x^2+\frac{c}{x^2}. \\
    \end{align*}

    To check this $y$, we differentiate,
    \[y'(x)=4x-\frac{2c}{x^3}.\]

    Then we compare, with the given differential equation where $y'$ is isolated,
    \begin{align*}
        4x-\frac{2c}{x^3}&=8x-\frac{2}{x}\left( 2x^2+\frac{c}{x^2} \right) \\
        &=8x-4x-\frac{2c}{x^3} \\
        &=4x-\frac{2c}{x^3}, \\
    \end{align*}
    which is true, so the general solution holds as well.

    \item $y'=xe^{y-x^2}, \quad y(0)=0$
    
    This is a separable differential equation. We also have an initial condition that will pin the single constant at a fixed number.

    We rewrite the equation with regards to differentials $\frac{dy}{dx}$, 
    \begin{align*}
        \frac{dy}{dx}&=\frac{xe^y}{e^{x^2}} \\
        \int\frac{dy}{e^y}&=\int\frac{x\,dx}{e^{x^2}} \\
        -e^{-y}&=-\frac{1}{2}\int e^u\,du \\
        e^{-y}&=\frac{1}{2}e^u+c \\
        e^{-y}&=\frac{1}{2}e^{-x^2}+c \\
        -y&=\ln{\left( \frac{1}{2}e^{-x^2}+c \right)} \\
        y&=-\ln{\left( \frac{1}{2}e^{-x^2}+c \right)}. \\
    \end{align*}

    We then consider the initial condition $y(0)=0$,
    \begin{align*}
        0&=-\ln{\left( \frac{1}{2}e^{-0^2}+c \right)} \\
        0&=-\ln{\left( \frac{1}{2}+c \right)} \\
        1&=\frac{1}{2}+c \\
        \frac{1}{2}=c. \\
    \end{align*}

    So, we have the solution,
    \begin{align*}
        y(x)&=-\ln{\left( \frac{1}{2}(1+e^{-x^2}) \right)} \\
        &=\ln{2}-\ln{\left( 1+e^{-x^2} \right)}. \\
    \end{align*}

    We can verify this solution in the same manner as previous problems.

    First, we differentiate our solution,
    \begin{align*}
        y'(x)&=\frac{d}{dx}\left[ \ln{2}-\ln{\left( 1+e^{-x^2} \right)} \right] \\
        &=-\frac{-2xe^{-x^2}}{1+e^{-x^2}} \\
        &=\frac{2x}{1+e^{x^2}}. \\
    \end{align*}

    Then we compare it to the given $y'$ with our derived solution $y$,
    \begin{align*}
        y'(x)&=\frac{xe^{\left( \ln{2}-\ln{\left( 1+e^{-x^2} \right)} \right)}}{e^{x^2}} \\
        &=\frac{xe^{\ln{2}}}{e^{x^2}e^{\ln{\left( 1+e^{-x^2} \right)}}} \\
        &=\frac{2x}{e^{x^2}\left( 1+e^{-x^2} \right)} \\
        &=\frac{2x}{1+e^{x^2}}. \\
    \end{align*}

    Since both $y'$ match, we confirm that we have arrived at a valid general solution.

    \item $(x+yx)\,dx=(x^2y^2+x^2+y^2+1)\,dy$
    
    We rearrange the terms to reveal that this equation is separable.
    \begin{align*}
        (x+yx)\,dx&=(x^2y^2+x^2+y^2+1)\,dy \\
        x(y+1)\,dx&=(x^2+1)(y^2+1)\,dy \\
        \int\frac{x\,dx}{x^2+1}&=\int\frac{y^2+1}{y+1}\,dy \\
        \frac{1}{2}\int\frac{du}{u}&=\int\frac{{(y+1)}^2-2y}{y+1}\,dy \\
        \frac{\ln{u}}{2}+c/2&=\int\left( y+1-\frac{2(y+1)-2}{y+1} \right)\,dy \\
        \frac{\ln{(x^2+1)}}{2}+c/2&=\int\left( y+1-2+\frac{2}{y+1} \right)\,dy\\
        &=\int\left(y-1+\frac{2}{y+1}\right)\,dy \\
        &=\frac{y^2}{2}-y+2\ln{(y+1)} \\
        \ln{(x^2+1)}+c&=y^2-2y+4\ln{(y+1)} \\
    \end{align*}

\end{enumerate}

\end{document}