\documentclass[../hw5]{subfiles}

\begin{document}

Find the first four Picard approximations of $y'=e^x+y$ with $y(0)=0$.

Since $y(x_0)=y_0$, then $(x_0,y_0)=(0,0)$.

So, $y_0(x)=y_0=0$.

The $n^{\text{th}}$ Picard approximation is given by
\[y_n(x)=y_0+\int_{x_0}^{x}f[x,y_{n-1}(x)]\,dx,\]
where $y'=f(x,y(x))$.

So, for $y_1$,
\begin{align*}
   y_1(x)&=0+\int_{0}^{x} f(x,y_0(x))\,dx \\
   &=\int_{0}^{x}(e^x+0)\,dx\\
   &=e^x\big\vert_{0}^{x} \\
   &=e^x-1. \\
\end{align*}

Next, for $y_2$,
\begin{align*}
    y_2(x)&=0+\int_{0}^{x}\left( e^x+(e^x-1) \right)\,dx \\
    &= \int_{0}^{x}(2e^x-1)\,dx \\
    &= {\left[ 2e^x-x \right]}_{0}^{x} \\
    &= 2e^x-x-2. \\
\end{align*}

For $y_3$,
\begin{align*}
    y_3(x)&=0+\int_{0}^{x}\left( e^x +(2e^x-x-2)\right)\,dx \\
    &= \int_{0}^{x}(3e^x-x-2)\,dx \\
    &= {\left[ 3e^x-\frac{x^2}{2}-2x \right]}_{0}^{x} \\
    &=3e^x-\frac{x^2}{2}-2x-3. \\
\end{align*}

Lastly, for $y_4$,
\begin{align*}
    y_4(x)&= 0+\int_{0}^{x}\left( e^x+\left( 3e^x-\frac{x^2}{2}-2x-3 \right) \right)\,dx \\
    &= \int_{0}^{x}\left( 4e^x-\frac{x^2}{2}-2x-3 \right)\,dx \\
    &= {\left[ 4e^x-\frac{x^3}{6}-x^2-3x \right]}_{0}^{x} \\
    &= 4e^x-\frac{x^3}{6}-x^2-3x-4. \\
\end{align*}

\end{document}