\documentclass[../hw6]{subfiles}
\begin{document}
\begin{problem}
With the same conditions as in Problem 1, prove \[
	\frac{1}{2\pi}\int_{-\pi}^{\pi} f(x)\overline{g(x)} \,dx = \sum_{-\infty}^{\infty} c_n \overline{d_n}
	.\]
\end{problem}
\begin{proof}
	Note that $f\overline{g}=\overline{f}g = 2\text{Re}(f\overline{g})$.

	By Problem 1, \[
		\sum_{-\infty}^{\infty} (c_n \overline{d_n} + \overline{c_n} d_n) = \frac{1}{2\pi}\int_{-\pi}^{\pi} 2\text{Re}(f\overline{g}) \,dx
		.\]

	Now, with $f=if$, we have \[
		\sum_{-\infty}^{\infty} (c_n \overline{d_n}- \overline{c_n}d_n) = \frac{1}{2\pi}\int_{-\pi}^{\pi} 2i \text{Im}(f\overline{g}) \,dx
		.\]

	So, summing both of the above, we have \[
		2 \sum_{-\infty}^{\infty} c_n \overline{d_n} = \frac{1}{\pi} \int_{-\pi}^{\pi} (\text{Re}(f\overline{g})+i\text{Im}(f\overline{g})) \,dx \implies \sum_{-\infty}^{\infty} c_n \overline{d_n} = \frac{1}{2\pi}\int_{-\pi}^{\pi} f(x)\overline{g(x)} \,dx
		.\]
\end{proof}
\end{document}
