\documentclass[../hw6]{subfiles}
\begin{document}
\begin{problem}
Find the Fourier series of the $2\pi$-periodic function $f_{\frac{\pi}{4}}(x)=\left( x-\frac{\pi}{4} \right) ^2$ on the interval $\left[ -\frac{3}{4}\pi,\frac{5}{4}\pi \right] $.
\end{problem}
\begin{proof}
	We will consider the Fourier series of $f_0(x)=x$ on $[-\pi,\pi]$ shifted by $x \to x-\frac{\pi}{4}$.
	Note that this substitution achieves both the desired function and interval.

	Since $f_0(x)=x^2$ is an even function, then its sine Fourier coefficients $b_n$ are zero.

	Then, for the constant term, \[
		\frac{1}{2}a_0=\frac{1}{2\pi}\int_{-\pi}^{\pi} x^2 \,dx = \frac{1}{3\pi}x^3\vert_0^{\pi}=\frac{\pi^2}{3}
		.\]

	Next, we have,
	\begin{align*}
		a_n & = \frac{1}{\pi} \int_{-\pi}^{\pi} x^2\cos{nx}  \,dx
		    & = \frac{2}{\pi}\left[ \frac{x^2\sin{nx}}{n}-\frac{2\sin{nx}}{n^3}+\frac{2x\cos{nx} }{n^2} \right]_0^{\pi} \\
		    & = 2\left( \frac{2\pi \cos{n\pi} }{n^2} \right)                                                            \\
		    & = \frac{4\cos{n\pi} }{n^2}                                                                                \\
		    & = \frac{ 4(-1)^n }{n^2}.
		.\end{align*}

	Therefore we have that \[
		f_0(x)=\frac{\pi^2}{3} + \sum_{n=1}^{\infty} \frac{4(-1)^n}{n^2}\cos{nx}
		.\]

	Now, shifting by $x\to x-\frac{\pi}{4}$, we have that \[
		f_{\frac{\pi}{4}}(x)=\frac{\pi^2}{3}+\sum_{n=1}^{\infty} \frac{4(-1)^n}{n^2}\cos{\left( n \left( x-\frac{\pi}{4} \right)  \right) }
		.\]
\end{proof}
\end{document}
