\documentclass[../hw6]{subfiles}
\begin{document}
\begin{problem}
Find the sum of the following series using the series for $x^2$ and choosing the appropriate value of $x$.
\begin{enumerate}
	\item $\sum_{1}^{\infty} \frac{1}{n^2}$.
	\item $\sum_{1}^{\infty} \frac{(-1)^{n+1}}{n^2}$.
\end{enumerate}
\end{problem}
From Problem 2, we have that, on $x \in [-\pi,\pi]$, \[
	f(x)=x^2=\frac{\pi^2}{3}+\sum_{1}^{\infty} \frac{4(-1)^n}{n^2}\cos{nx}
	.\]
\begin{proof}[Proof of (i)]
	If $x=\pi$, then $\cos{nx}=(-1)^n$.
	So, since $f$ is continuous at  $\pi$,  \[
		f(\pi)=\pi^2=\frac{\pi^2}{3}+\sum_{1}^{\infty} \frac{4(-1)^n}{n^2}(-1)^n \implies \frac{\pi^2}{6} = \sum_{1}^{\infty} \frac{1}{n^2}
		.\]
\end{proof}
\begin{proof}[Proof of (ii)]
	Since $f$ is continuous at zero and $x=0\implies \cos{nx}=1$, then \[
		f(0)=0 = \frac{\pi^2}{3}+\sum_{1}^{\infty} \frac{4(-1)^n}{n^3} \implies \frac{\pi^2}{12}=\sum_{1}^{\infty} \frac{(-1)^{n+1}}{n^2}
		.\]
\end{proof}
\end{document}
