\documentclass[../hw7]{subfiles}

\begin{document}

Solve \[y''+'=f(t), \quad y(0)=y'(0)=0,\] where \[f(t)=\begin{cases}
    4, & 0\leq t \leq 2, \\
    t+2, & 2<t. \\
\end{cases}\]

First, we rewrite the piecewise function $f$ using the step function $H$, where
\[H(t) = \begin{cases} 
    0 & \text{if } t < 0,\\
    1 & \text{if } t \geq 0;
\end{cases}
\] we will use $H_c=H(t-c)$.

The forcing function becomes
\begin{align*}
    f(t)&=4(1-H_2)+(t+2)H_2 \\
    &= 4+(t+2-4)H_2 \\
    &= 4+(t-2)H_2. \\
\end{align*}

Let $\lapl{y}=Y$. Then, the Laplace transform of 
\[y''+y=4+(t-2)H_2\]
becomes 
\begin{align*}
    s^2Y-sy(0)-y'(0)+Y&=\frac{4}{s}+\frac{e^{-2s}}{s^2}\\
    (s^2+1)Y&=\frac{4}{s}+\frac{e^{-2s}}{s^2}\\
    Y&=\frac{4}{s(s^2+1)}+\frac{e^{-2s}}{s^2(s^2+1)}.\\
\end{align*}

Let us take a moment to consider the partial fraction expansions of $\frac{1}{s(s^2+1)}$ and $\frac{1}{s^2(s^2+1)}$.
We will show that the following hold:

first, 
\begin{align*}
    \frac{1}{s(s^2+1)}&=\frac{1}{s}-\frac{s}{s^2+1}\\
    &=\frac{s^2+1}{s(s^2+1)}-\frac{s^2}{s(s^2+1)}\\
    &=\frac{1}{s(s^2+1)}.\\
\end{align*}

Next,
\begin{align*}
    \frac{1}{s^2(s^2+1)}&=\frac{1}{s^2}-\frac{1}{s^2+1}\\
    &=\frac{s^2+1}{s^2(s^2+1)}-\frac{s^2}{s^2(s^2+1)}\\
    &=\frac{1}{s^2(s^2+1)}.\\
\end{align*}

We continue from above, substituting the partial fractions in place of the product denominators,
\[Y=4\left( \frac{1}{s}-\frac{s}{s^2+1} \right)+e^{-2s}\left( \frac{1}{s^2}-\frac{1}{s^2+1} \right).\]

We find the general solution $y$ by taking the inverse Laplace transform,
\[y=4(1-\cos{t})+H_2\left( (t-2)-\sin{(t-2)} \right).\]


\end{document}
