\documentclass[../hw7]{subfiles}

\begin{document}

Compute the inverse Laplace transform of the following functions.

\begin{enumerate}[label= (\alph*)]
    \item \begin{enumerate}[label= (\roman*)]
        \item \[\begin{WithArrows}
            F_1(s) &= \frac{1}{s^2+2s+10} \\
            &= \frac{1}{{(s+1)}^2+3^2} \Arrow{$\mathcal{L}^{-1}$} \\
            &=\frac{1}{3}e^{-t}\sin{3t}.
        \end{WithArrows}\]

        \item \[\begin{WithArrows}
            F_2(s) &= \frac{3s}{s^2+4s+13} \\
            &=\frac{3(s+2)-6}{{(s+2)}^2+3^2} \\
            &= 3\frac{s+2}{{(s+2)}^2+3^2}-2\frac{3}{{(s+2)}^2+3^2}\Arrow{$\mathcal{L}^{-1}$} \\
            &= e^{-2t}(3\cos{3t}-2\sin{3t}).
        \end{WithArrows}\]

        \item \[\begin{WithArrows}
            F_3(s)&=\frac{2s+7}{s^2+6s+9} \\
            &= \frac{2(s+3)+1}{{(s+3)}^2} \\
            &= \frac{2}{s+3}+\frac{1}{{(s+3)}^2}\Arrow{$\mathcal{L}^{-1}$} \\
            &= e^{-3t}(t+2).
        \end{WithArrows}\]
    \end{enumerate}

    \item \begin{enumerate}[label= (\roman*)]
        \item \[\begin{WithArrows}
            F_1(s)&= \frac{s^2-6}{s^3+4s^2+3s} \\
            &= \frac{s^2-6}{s(s+1)(s+3)} \\
            &= \frac{-6/3}{s}+\frac{-5/2}{s+1}+\frac{3/6}{s+3} \\
            &= \frac{1}{6}\left( \frac{3}{s+3}-\frac{-15}{s+1}-\frac{12}{s} \right) \Arrow{$\mathcal{L}^{-1}$} \\
            &= \frac{1}{6}\left( 3e^{-3t}-15e^{-t}-12 \right) \\
            &= \frac{1}{2}e^{-3t}-\frac{5}{2}e^{-t}-2t.
        \end{WithArrows}\]

        \item \[\begin{WithArrows}
            F_2(s)&= \frac{16}{s(s^2+4)}\\
            &= 4\left( \frac{1}{s}-\frac{s}{s^2+4} \right)\Arrow{$\mathcal{L}^{-1}$} \\
            &= 4\left( 1-\cos{2t} \right).
        \end{WithArrows}\]

        \item \[\begin{WithArrows}
            F_3(s)&= \frac{6s-3}{s{(s+1)}^2}\\
            &= 3\left( \frac{-1}{s}+\frac{(s+1)+3}{{(s+1)}^2} \right) \\
            &= 3\left( \frac{3}{{(s+1)}^2}+\frac{1}{s+1}-\frac{1}{s} \right) \Arrow{$\mathcal{L}^{-1}$} \\
            &= 3(3te^{-t}+e^{-t}-1) \\
            &= 3e^{-t}(3t+1-e^t).
        \end{WithArrows}\]
    \end{enumerate}

    \item \[\begin{WithArrows}
        F(s)&= \frac{(1-e^{-2s})(1-3e^{-2s})}{s^2} \\
        &= \frac{1-4e^{-2s}+3e^{-4s}}{s^2} \\
        &= \frac{1}{s^2}-4\frac{e^{-2s}}{s^2}+3\frac{e^{-4s}}{s^2}\Arrow{$\mathcal{L}^{-1}$} \\
        &= t+3(t-4)H_4-4(t-2)H_2.
    \end{WithArrows}\]
\end{enumerate}

\end{document}
