\documentclass[../root file]{subfiles}

\begin{document}

Prove that $\sum_{k=1}^{\infty} (a_{k+1}-a_k)$ converges iff $a_n$ converges.



\begin{proof}
    $(\implies)$ Let $\sum (a_{k+1}-a_k)$ converge to $L$.

    So, \[\lim\limits_{n\to\infty} \sum_{k=1}^{n} (a_{k+1}-a_k) = L.\]

    Then,
    \begin{align*}
        L &= \lim\limits_{n\to\infty} \left[\sum_{k=1}^{n} a_{k+1}- \sum_{k=1}^{n} a_k\right]\\
        &= \lim\limits_{n\to\infty} \left[\sum_{k=2}^{n+1} a_{k} - \sum_{k=1}^{n} a_k\right]\\
        &= \lim\limits_{n\to\infty} \left[a_{n+1} + \sum_{k=2}^{n} a_{k} - \left(\sum_{k=2}^{n} a_k + a_1\right)\right]\\
        &= \lim\limits_{n\to\infty} [a_{n+1}-a_1]\\
        L+a_1 &= \lim\limits_{n\to\infty} a_{n+1} \\
        L+a_1 &= \lim\limits_{n\to\infty} a_n. \\
    \end{align*}

    So, $a_n$ converges.

    $(\impliedby)$ Let $(a_n)$ converge to $L$; Since $a_n\to L$, then $a_{n+1}\to L$ as well.

    We compute the sum,
    \begin{align*}
        \sum_{k=1}^{\infty}(a_{k+1}-a_k)&=\sum_{k=1}^{\infty} a_{k+1} - \sum_{k=1}^{\infty} a_k \\
        &= \lim\limits_{n\to\infty} \left[ \sum_{k=1}^{n} a_{k+1} - \sum_{k=1}^{n} a_k \right] \\
        &= \lim\limits_{n\to\infty} \left[ \sum_{k=2}^{n+1} a_k - \sum_{k=1}^{n} a_k \right] \\
        &= \lim\limits_{n\to\infty} \left[ a_{n+1} \sum_{k=2}^{n} a_k - \left(\sum_{k=2}^{n} a_k + a_1\right) \right] \\
        &= \lim\limits_{n\to\infty} [a_{n+1}-a_1] \\
        &= \lim\limits_{n\to\infty} a_{n+1} - a_1 \\
        &= L-a_1.
    \end{align*}

    So, the sum also converges.
\end{proof}

\end{document}