\documentclass[../hw1]{subfiles}
\begin{document}
\begin{problem}[6]
Let $f(x)=x^2(x-\sin{x})$ and $g(x)=(e^{x}-1){(\cos{2x}-1 )}^2$.
\begin{enumerate}[label=\alph*)]
	\item Compute $T_5$ at  $x_0=0$.

	      With the fifth order Taylor polynomial of sine, $\sum_{j=0}^{5} \frac{(-1)^j x^{2j+1}}{(2j+1)!}$,
	      \begin{align*}
		      T_5(f) & = x^2\left( x - \left( x-\frac{x^3}{3!} + \frac{x^5}{5!} - \frac{x^7}{7!} + \frac{x^9}{9!} - \frac{x^{11}}{11!} \right)  \right) \\
		             & = \frac{x^5}{3!} - \frac{x^7}{5!} + \frac{x^9}{7!} - \frac{x^{11}}{9!} + \frac{x^{13}}{11!}
		      .\end{align*}

	      Then, using the expansions of cosine and the exponential function,
	      \begin{align*}
		      T_5(g) & = \left( \sum_{0}^{5} \frac{x^k}{k!}-1  \right) {\left( \sum_{0}^{5} \frac{(-1)^k {(2x)}^{2k}}{(2k)!} -1\right)}^2 \\
		             & = \left( \sum_{0}^{5} \frac{x^k}{k!}  \right) {\left( \sum_{1}^{5}  \frac{(-1)^k {(2x)}^{2k}}{(2k)!}\right) }^2
		      .\end{align*}

	      Since each of the leading terms in both sums if one, then we can expand the above to,
	      \[
		      \left( x + \frac{x^2}{2} + \frac{x^3}{3!} + \frac{x^4}{4!} + \frac{x^5}{5!} \right) \left( - 2x^2 + \frac{2x^4}{3} - \frac{{(2x)}^6}{6!}  +  \frac{{(2x)}^8}{8!} - \frac{{(2x)}^{10}}{10!}\right)
		      .\]

	\item Use (a) to find $\lim_{x \to \infty} \frac{f(x)}{g(x)}$ without L'Hopital.

	      To consider $x\to \infty$, we will use the largest order terms.

	      From $f$, this is  $\frac{x^{13}}{11!}$.
	      From $g$, this is $\frac{x^5}{5!}\left( -\frac{{(2x)}^{10}}{10!} \right) = \frac{-2^{10} x^{15}}{5! 10!}$

	      So $\frac{f}{g} = O(\frac{1}{x^2})$, which goes to zero as $x\to \infty$.
	      Thus, $\lim_{x \to \infty} \frac{f(x)}{g(x)} = 0$ as well.
\end{enumerate}
\end{problem}
\end{document}
