\documentclass[../hw3]{subfiles}
\begin{document}
\begin{problem}
$kI = \begin{pmatrix} k & 0 \\ 0 & k \end{pmatrix} ,\, k\in \R$ is a scalar matrix.
\begin{enumerate}[label=\alph*)]
	\item Prove that the set of scalar matrices is a subring of $M(\R)$.
	\item Show that $\forall A\in M(\R),\, KA=AK$ where $K$ is a scalar matrix.
	\item  Show that, for $K\in M(\R),\, \forall A\in M(\R),\, KA=AK \implies K$ is a scalar matrix.
\end{enumerate}
\end{problem}
\begin{proof}[Proof of a]
	First, we see that $\forall k\in \R,\,  kI \subset M(\R)$.

	Next, scalar matrices are closed under addition, have a zero element, and have an additive inverse as in $\R$.

	Since we can write scalar matrices as $kI$ where  $I$ is the identity matrix, then products are of the form  $(aI)(bI)=(ab)(II)=(ab)I$.
	So, scalar matrices are closed under multiplication.

	Therefore, the set of scalar matrices forms of subring of $M(\R)$.
\end{proof}

\begin{proof}[Proof of b]
	Let $K=kI$ where  $k\in \R$ and $I$ is the $2\times 2$ identity matrix.

	Then, \[
		KA=(kI)A = k(IA) = kA = k(AI) = A(kI) = AK
		.\]
\end{proof}

\begin{proof}[Proof of c]
	Let $K = \begin{pmatrix} a & b \\ c & d \end{pmatrix} $.
	First, let $A=\begin{pmatrix} 1 & 0 \\ 0 & 0 \end{pmatrix} $

	Then,
	\begin{align*}
		KA    & = \begin{pmatrix} a & b \\ c & d \end{pmatrix}\begin{pmatrix} 1 & 0 \\ 0 & 0 \end{pmatrix} = \begin{pmatrix} a & 0 \\ c & 0 \end{pmatrix} \\
		AK    & = \begin{pmatrix} 1 & 0 \\ 0 & 0 \end{pmatrix} \begin{pmatrix} a & b \\ c & d \end{pmatrix}= \begin{pmatrix} a & b \\ 0 & 0 \end{pmatrix} \\
		KA=AK & \implies \begin{pmatrix} a & 0 \\ c & 0 \end{pmatrix} = \begin{pmatrix} a & b \\ 0 & 0 \end{pmatrix}                                      \\
		      & \implies b = 0 \land c = 0
		.\end{align*}

	Now, let $A = \begin{pmatrix} 0&1\\0&0 \end{pmatrix} $.
	\begin{align*}
		KA    & = \begin{pmatrix} a & b \\ c & d \end{pmatrix}\begin{pmatrix} 0&1 \\ 0 & 0 \end{pmatrix} = \begin{pmatrix} 0&a \\ 0&c \end{pmatrix}   \\
		AK    & = \begin{pmatrix} 0&1 \\ 0 & 0 \end{pmatrix} \begin{pmatrix} a & b \\ c & d \end{pmatrix}= \begin{pmatrix} c&d \\ 0 & 0 \end{pmatrix} \\
		KA=AK & \implies \begin{pmatrix} 0&a \\ 0&c \end{pmatrix} = \begin{pmatrix} c&d \\ 0 & 0 \end{pmatrix}                                        \\
		      & \implies a=d
		.\end{align*}

	Therefore, $K= \begin{pmatrix} a&0\\0&a \end{pmatrix} =aI$, which is a scalar matrix.
\end{proof}
\end{document}
