\documentclass[../hw8]{subfiles}

\begin{document}

Find the general solution to $(1+t^2)y''-4ty'+6y=0$ using the series method.

First, we rewrite the equation using series,
\[\sum\limits_{k=2}^{\infty}k(k-1)a_k t^{k-2}+\sum\limits_{k=2}^{\infty}k(k-1)a_k t^k - 4 \sum\limits_{k=1}^{\infty}ka_k t^k + 6 \sum\limits_{k=0}^{\infty}a_k t^k=0.\]

Then, we shift each term to match in the power of $t$,
\[\sum\limits_{m=0}^{\infty}(m+2)(m+1)a_{m+2}t^m+\sum\limits_{k=2}^{\infty}m(m-1)a_m t^m-4 \sum\limits_{m=1}^{\infty}ma_m t^m+6 \sum\limits_{m=0}^{\infty}a_m t^m=0.\]

Next, we start all summations at the latest index $m=2$ by bringing out prior terms,
\[2a_2+6a_3t-4a_1t+6a_0+6a_1t+\sum\limits_{m=2}^{\infty}\left[ (m+2)(m+1)a_{m+2}+m(m-1)a_m-4ma_m+6a_m \right]t^m=0.\]

We will first confider the initial coefficients by separating them into their respective powers of $t$, $t^0$ and $t^1$.

Recalling that the equation is identically for all $t$, we see that,
\begin{align*}
    2a_2+6a_0&=0\\
    a_2&=-3a_0;\\
\end{align*}
\begin{align*}
    (6a_3-4a_1+6a_1)t&=0\\
    (6a_3+2a_1)t&=0\\
    a_3&=-\frac{a_1}{3}.\\
\end{align*}

We proceed with the recursive relation,
\begin{align*}
    (m+2)(m+1)a_{m+2}+m(m-1)a_m-4ma_m+6a_m&=0\\
    a_{m+2}&=-\frac{m(m-1)-4m+6}{(m+1)(m+2)}a_m\\
    &=-\frac{m^2-5m+6}{(m+1)(m+2)}a_m\\
    &=-\frac{(m-2)(m-3)}{(m+1)(m+2)}a_m.\\
\end{align*}

We will evaluate a few terms to see that, for $n\geq4$, all coefficients $a_n=0$.

For $m=2$, \[a_4=-\frac{(2-2)(2-3)}{(2+1)(2+2)}a_2=0.\]

For $m=3$, \[a_5=-\frac{(3-2)(3-3)}{(3+1)(3+2)}a_3=0.\]

Since all higher coefficients are multiples of $a_4$ and $a_5$, then they are all zero.

So, we are left with \[a_0+a_1t+a_2t^2+a_3t^3,\]
which can be expressed from the two arbitrary constants--from the second order differential equation--$a_0$ and $a_1$, \[a_0+a_1t-3a_0t^2-\frac{a_1t^3}{3}.\]

We relabel using $a_0=c_1$ and $a_1=c_2$ and collect terms,
\[y(t)=c_1(1-3t^2)+c_2\left( t-\frac{t^3}{3} \right).\]



\end{document}
