\documentclass{article}
\begin{document}
Let $n$ and $k$ be positive integers with $k \le n$. Prove that
\[
	\sum_{i=0}^k \binom{n}{i}(-1)^i = \binom{n-1}{k}(-1)^k.
\]
\begin{proof}
	By the alternating sum identity, we have
	\begin{align*}
		0=\sum_{i=0}^{n} \binom{n}{i} (-1)^i = & \sum_{i=0}^{k} \binom{n}{i} (-1)^i+\sum_{i=k+1}^{n} \binom{n}{i} (-1)^i     \\
		\implies                               & \sum_{i=0}^{k} \binom{n}{i} (-1)^i = - \sum_{i=k+1}^{n} \binom{n}{i} (-1)^i
		.\end{align*}

	By the Pascal's triangle summation identity, we have
	\[
		\binom{n}{i}= \binom{n-1}{i-1}+\binom{n-1}{i}
		.\]

	So,
	\begin{align*}
		\sum_{i=k+1}^{n} \binom{n}{i} (-1)^i & = \sum_{i=k+1}^{n} \left[ \binom{n-1}{i-1}+\binom{n-1}{i} \right](-1)^i             \\
		                                     & = \sum_{i=k+1}^{n} \binom{n-1}{i-1} (-1)^i + \sum_{i=k+1}^{n} \binom{n-1}{i} (-1)^i
		.\end{align*}

	We will reindex the left sum by $i=j + 1$ and split off the first summand on the left and then final summand on the right term; the above becomes,
	\begin{align*}
		 & = \sum_{j=k}^{n-1} \binom{n-1}{j} (-1)^{j+1}+\left( \sum_{i=k+1}^{n} \binom{n-1}{i} (-1)^i + \binom{n-1}{n}(-1)^n \right)                        \\
		 & = -\left( \binom{n-1}{k}(-1)^k + \sum_{j=k+1}^{n-1} \binom{n-1}{j} (-1)^{j+1}\right) + \left( \sum_{i=k+1}^{n} \binom{n-1}{i} (-1)^i + 0 \right) \\
		 & = -\binom{n-1}{k}(-1)^k
		.\end{align*}

	So, \[
		\sum_{i=0}^{k} \binom{n}{i} (-1)^k = -\sum_{i=k+1}^{n} \binom{n}{i} (-1)^k = \binom{n-1}{k}(-1)^k
		.\]
\end{proof}
\end{document}
