\documentclass[../hw7]{subfiles}

\begin{document}

Compute the sawtooth function $\lapl{h(t)}$, where \[h(t)=\begin{cases}
    t, & 0\leq t < 1, \\
    h(t-1), & 1 \leq t. \\
\end{cases}\]

We begin by writing $h$ in terms of the step function $H$,
\[h(t)=t(1-H_1)+h(t-1)H_1.\]

We then take the Laplace transform of this equation with the fact that \[\lapl{f(t-c)H_c}=e^{-cs}\lapl{f(t)},\]
\begin{align*}
    \lapl{h(t)}&=\frac{1}{s^2}-e^{-s}\left( \frac{1}{s^2}+\frac{1}{s} \right)+e^{-s}\lapl{h(t)} \\
    (1-e^{-s})\lapl{h(t)}&=\frac{1-e^{-s}}{s^2}-\frac{e^{-s}}{s} \\
    \lapl{h(t)}&=\frac{1}{s^2}-\frac{e^{-s}}{s\left( 1-e^{-s} \right)} \\
    \lapl{h(t)}&=\frac{1}{s^2}-\frac{1}{s\left( e^s-1 \right)}. \\
\end{align*}

\end{document}
