\documentclass[../hw7]{subfiles}

\begin{document}

Compute the Laplace transform of each of the following functions.
\begin{enumerate}[label= (\alph*)]
    
    \item \begin{enumerate}[label= (\roman*)]
        
        \item $f_1(t)=te^{4t}\cos{(-2t)}$
        First, take \[\lapl{t\cos{(-2t)}}=\frac{s^2-4}{{(s^2+4)}^2},\] then shift the Laplace function in the frequency domain by the exponential $e^{4t}$ so that we obtain, \[\lapl{te^{4t}\cos{(-2t)}}=\frac{{(s-4)}^2-4}{{\left( {(s-4)}^2+4 \right)}^2}.\]
        
        \item $f_2(t)=\cos^2{t}$
        We will use the identity, \[\cos^2{t}=\frac{1+\cos{2t}}{2}.\]
        
        So,
        \begin{align*}
            \lapl{\cos^2{t}}&=\lapl{\frac{1}{2}(1+\cos{2t})} \\
            &= \frac{1}{2}\left[ \lapl{1}+\lapl{\cos{2t}} \right] \\
            &= \frac{1}{2}\left( \frac{1}{s}+\frac{s}{s^2+4} \right). \\
        \end{align*}

        \item $f_3(t)=\sqrt{t}e^t$
        We will consider $\lapl{\sqrt{t}}$ shifted by $e^t$.
        Given that \[\lapl{\sqrt{t}}=\frac{1}{2}\sqrt{\frac{\pi}{s^3}},\]
        then, \[\lapl{\sqrt{t}e^t}=\frac{1}{2}\sqrt{\frac{\pi}{{(s-1)}^3}}.\]

    \end{enumerate}
    
    \item $f(t)=\begin{cases}
        4, & t<2, \\
        t+2, & 2\leq t \leq 5, \\
        e^{-t}, & 5<t. \\
    \end{cases}$

    We begin by rewriting the piecewise function in terms of the step function $H$, where $H_c(t)=H(t-c)$.

    So,
    \begin{align*}
        f(t)&=4(1-H_2)+(t+2)(H_2-H_5)+e^{-t}H_5\\
        &=t+(t+2-4)H_2+(e^{-t}-t-2)H_5\\
        &=4+(t-2)H_2-(t-5)H_5+(e^{-t}-7)H_5.\\
    \end{align*}

    The Laplace transform of $f$ is then, 
    \begin{align*}
        \lapl{f}&=\frac{4}{s}+\frac{e^{-2s}}{s^2}-\frac{e^{-5s}}{s^2}+e^{-5s}\lapl{e^{-(t+5)}+7}\\
        &=\frac{4}{s}+\frac{e^{-2s}}{s^2}-\frac{e^{-5s}}{s^2}+e^{-5s}\left( \frac{e^5}{s+1}+\frac{7}{s} \right) \\
        &=\frac{4+7e^{-5s}}{s}+\frac{e^{-2s}-e^{-5s}}{s^2}+\frac{e^{5(1-s)}}{s+1}. \\
    \end{align*}

\end{enumerate}

\end{document}
