\documentclass[../hw5]{subfiles}
\begin{document}
\begin{problem}
\begin{enumerate}
	\item The square wave $f(x)=\begin{cases}
			      -1 & (-\pi,0 ), \\ 1 & (0,\pi ).
		      \end{cases}$
	\item $f(x)=\sin^2{x}$.
\end{enumerate}
\end{problem}
\begin{proof}[Proof of (i)]
	We have that $f$ is an odd function, so  $a_n=0$ for all  $n$.

	We will proceed to find the $b_n$ Fourier coefficients,
	\begin{align*}
		b_n & = \frac{1}{\pi }\int_{-\pi }^{\pi }f(x)\sin{nx} \,dx                                         \\
		    & = \frac{1}{\pi}\int_{0}^{\pi } \sin{nx} \,dx - \frac{1}{\pi }\int_{-\pi }^{0} \sin{nx}  \,dx \\
		    & = \frac{2}{\pi }\int_{0}^{\pi } \sin{nx}  \,dx                                               \\
		    & = \frac{2}{\pi }\left[ -\frac{\cos{nx} }{n} \right]^{\pi }_0                                 \\
		    & = \frac{2}{\pi }\left( \frac{1-\cos{n\pi } }{n} \right)
		,\end{align*}
	which vanishes for all even $n$, and is $\frac{4}{n\pi}$ for all odd $n$.

	Thus, we have that, for $n$ odd, \[
		f(x)=\sum_{n=1}^{\infty} \frac{4}{\pi }\frac{\sin{nx}}{n}
		,\] which is \[
		\sum_{k=0}^{\infty} \frac{4\sin{(2k+1)x}}{\pi(2k+1) }
		.\]
\end{proof}
\begin{proof}[Proof of (ii)]
	We have that \[
		f(x)=\sin^2{x}=\frac{1-\cos{2x} }{2}=\frac{1}{2}-\frac{1}{2}\cos{2x}
		.\]
\end{proof}
\end{document}
