\documentclass[../hw5]{subfiles}
\begin{document}
\begin{problem}
\begin{enumerate}
	\item Prove \[
		      \sum_{k=0 }^{n-1} \sin{\left( k+\frac{1}{2} \right) x } = \frac{\sin^2{\left( \frac{nx}{2} \right) } }{\sin{(\frac{x}{2})} },\quad \forall n\ge 1
		      .\]
	\item Use (i) to show \[
		      \int_{0}^{\pi} \frac{\sin^2{\left( \frac{nx}{2} \right) } }{\sin{\left( \frac{x}{2} \right) } } \,dx = \pi, \quad \forall n\ge 1
		      .\]
\end{enumerate}
\end{problem}
\begin{proof}[Proof of (i)]
	We will induct on $n$.

	For $n=1$,  \[
		\sum_{k=0}^{1-1=0} \sin{\left( \frac{2k+1}{2}x \right) } = \sin{\frac{x}{2}} = \frac{\sin^2{\frac{x}{2}} }{\sin{\frac{x}{2}} }
		.\]

	Assume that (i) holds for $n$.
	Now, for $n+1$, \[
		\sum_{k=0 }^{n} \sin{\frac{2k+1}{2}x} = \frac{\sin^2{\frac{nx}{2}}}{\sin{\frac{x}{2}} }+\sin{\frac{2n+1}{2}x}
		.\]

	Consider the right summand; using the product of sines,
	\begin{align*}
		\frac{\sin{\left(\frac{2n+1}{2}\right)x}\cdot \sin{\frac{x}{2}}  }{\sin{\frac{x}{2}} }
		 & = \frac{1}{2\sin{\frac{x}{2}} }\left( \cos{\left( \frac{2n+1}{2}-\frac{1}{2} \right)x } - \cos{ \left( \frac{2n+1}{2}+\frac{1}{2} \right) x}  \right) \\
		 & = \frac{1}{2\sin{\frac{x}{2}} }\left( \cos{nx}-\cos{(n+1)x}   \right)
		.\end{align*}
	Then, for left summand, using square sine identity, \[
		\frac{\sin^2{\frac{nx}{2}}}{\sin{\frac{x}{2}} } = \frac{1-\cos{nx} }{2\sin{\frac{x}{2}} }
		.\]

	So, the above sum in the inductive step simplifies to, \[
		\frac{1-\cos{(n+1)x} }{2\sin{\frac{x}{2}} } = \frac{\sin^2{\left(\frac{n+1}{2}\right)x} }{\sin{\frac{x}{2}} }
		,\] which is our desired result with $n+1$.
\end{proof}
\begin{proof}[Proof of (ii)]
	We will induct on $n$.

	For $n=1$,  \[
		\int_{0}^{\pi} \frac{\sin^2{\frac{x}{2}} }{\sin^2{\frac{x}{2}}} \,dx = \int_{0}^{\pi} dx = 1\cdot \pi
		.\]

	Assume (ii) holds for $n$.
	Now, for $n+1$, by part (i), \[
		\int_{0}^{\pi} \frac{\sin^2{\left( \frac{n+1}{2} \right) x} }{\sin^2{\frac{x}{2}} } \,dx
		= \int_{0}^{\pi} \sum_{k=0}^{n} \frac{\sin{\left( k+\frac{1}{2} \right) x} }{\sin{\frac{x}{2}} } \,dx
		= \sum_{k=0}^{n} \int_{0}^{\pi} \frac{\sin{\left( k+\frac{1}{2} \right) x} }{\sin{\frac{x}{2}} } \,dx
		.\]

	Here, we have the $k^{\text{th}}$ Dirichlet kernel $D_k(x)$, where \[
		D_k(x)=\frac{\sin{\left( k+\frac{1}{2} \right) x} }{2\pi\sin{\frac{x}{2}} },
		\quad \int_{0}^{\pi} D_k(x) \,dx = \frac{1}{2}
		.\]

	So, the above is \[
		\sum_{k=0 }^{n} \int_{0}^{\pi} 2\pi D_k(x) \,dx = \sum_{0}^{n} 2\pi\cdot \frac{1}{2} = n\pi
		.\]
\end{proof}
\end{document}
