\documentclass[..hw1]{subfiles}
\begin{document}
\begin{problem}
Let $x,y\in \R^{n}$. \begin{enumerate}[label=\alph*)]
	\item Prove $2\left( {|x|}^2+{|y|}^2 \right) = {|x+y|}^2+{|x-y|}^2$.
	      \begin{proof}[Proof]
		      First, we will expand ${|x+y|}^2$,
		      \begin{align*}
			      {|x+y|}^2 & = \inp{x+y}{x+y}                              \\
			                & = \inp{x}{x+y}+\inp{y}{x+y}                   \\
			                & = \inp{x}{x}+\inp{x}{y}+\inp{y}{x}+\inp{y}{y} \\
			                & = {|x|}^2+2\inp{x }{y }+{|y|}^2.              \\
		      \end{align*}

		      We will do the same for ${|x-y|}^2$,
		      \begin{align*}
			      {|x-y|}^2 & = \inp{x-y}{x-y}                                      \\
			                & = \inp{x }{x-y }-\inp{y }{x-y }                       \\
			                & = \inp{x }{x }-\inp{x }{y }-\inp{y }{x }+\inp{y }{y } \\
			                & = {|x|}^2-2\inp{x }{y }+{|y|}^2.                      \\
		      \end{align*}

		      So, combining these, \[
			      {|x+y|}^2+{|x-y|}^2=2\left( {|x|}^2+{|y|}^2 \right)
			      ,\] as desired.
	      \end{proof}
	\item Prove the polarization identity, $\inp{x}{y}=\frac{{|x+y|}^2-{|x-y|}^2}{4}$.
	      \begin{proof}
		      We note that, with the commutativity of the inner product,
		      \begin{align*}
			      \inp{a+b}{a+b} & = \inp{a}{a+b}+\inp{b}{a+b}                     \\
			                     & = \inp{a}{a} + \inp{a}{b}+\inp{b}{a}+\inp{b}{b} \\
			                     & = \inp{a}{a}+2\inp{a}{b}+\inp{b}{b}.            \\
		      \end{align*}

		      Furthermore, scalars distribute over the inner product. For $x,y\in \R^{n},\ a\in \R$, \[
			      \inp{x}{ay} = a\inp{x}{y} = \inp{ax}{y}
			      .\]

		      So, $\inp{x-y}{x-y} = \inp{x}{x} - 2\inp{x}{y} + \inp{y}{y}$.

		      So, the identity can expand,
		      \begin{align*}
			      \inp{x}{y} & =\frac{1}{4}\left( \inp{x+y}{x+y}-\inp{x-y}{x-y} \right)                                                              \\
			                 & = \frac{1}{4} \left( \inp{x}{x}+2\inp{x}{y}+\inp{y}{y} \right) - \left( \inp{x}{x} - 2\inp{x}{y} + \inp{y}{y} \right) \\
			                 & = \frac{1}{4}\left( 4\inp{x}{y} \right)                                                                               \\
			                 & = \inp{x}{y},                                                                                                         \\
		      \end{align*}
		      as desired.
	      \end{proof}

\end{enumerate}
\end{problem}
\end{document}
