\documentclass{article}
\begin{document}
\begin{problem}
Show $x_1,\ldots,x_m\in \R^n$ and $\forall i\neq j.\  \inp{x_{i}}{x_{j}}=0  \implies {|x_1+\cdots+x_{m}|}^2={|x_1|}^2+\cdots+{|x_m|}^2$.
\end{problem}
\begin{proof}
	We will prove the statement by induction on $m\in \Z^+$.

	For the base case, when $m=2,\ \inp{x_1}{x_2}=0$,
	\begin{align*}
		{x_1+x_2}^2 & = \inp{x_1+x_2}{x_1+x_2}              \\
		            & = {|x_1|}^2+2\inp{x_1}{x_2}+{|x_2|}^2 \\
		            & = {|x_1|}^2+{|x_2|}^2
		.\end{align*}

	We will assume that the $m=k$ case holds by the Inductive Hypothesis,  \[
		{|x_1+\cdots+x_{m}|}^2={|x_1|}^2+\cdots+{|x_m|}^2
		.\]

	Then, for the following $m=k+1$ case, \[
		{|x_1+\cdots+x_{m}+x_{m+1}|}^2 = \inp{x_1+\cdots+x_{m}+x_{m+1 }}{x_1+\cdots+x_{m}+x_{m+1}}
		.\]
	We distribute only the ${x_{m+1}}^{\text{th}}$ term, \[
		{|x_1+\cdots+x_{m}+x_{m+1}|}^2 = \inp{x_1+\cdots+x_{m}}{x_1+\cdots+x_{m}}+2\inp{x_{m+1}}{x_1+\cdots+x_{m}}+\inp{x_{m+1}}{x_{m+1}}
		.\]

	We see that the first term becomes ${|x_1|}^2+\cdots+{|x_{m}|}^2$ by the I.H., and that the last term is ${|x_{m+1}|}^2$.
	Now, for the middle term, if we distribute $x_{m+1}$ across the right hand side of the inner product, we will be left with inner products of the form $\inp{x_{m+1}}{x_{i}}$ where $1\le i \le m$.
	However, $m+1\neq i$ for all such $i$.
	Therefore, by the problem statement, the middle term must be zero.

	Thus, \[
		{|x_1+\cdots+x_{m+1}|}^2={|x_1|}^2+\cdots+{|x_m+1|}^2
		.\]

	Since the base case $m=2$ holds, and the inductive case  $m=k+1$ holds when  $m=k$ holds, then the statement is true for all  $m\in \Z^+$.

\end{proof}
\end{document}
