\documentclass[../hw8]{subfiles}

\begin{document}

\subsection*{66}
Find a formula for the $n$th derivative.
\[\frac{d^n}{dx^n}[\ln{(1-x)}]\]

\begin{proposition}
    $\frac{d^n}{dx^n}[\ln{(1-x)}] = (n-1)!{(-1)}^n{(1-x)}^{-n}$.
\end{proposition}

\begin{proof}
    We will prove that the proposition holds by induction on $n$.

    For the base case, when $n=1$,
    \[(1-1){(-1)}^1{(1-x)}^{-1}=\frac{-1}{1-x}.\]

    We verify by differentiating $\ln{(1-x)}$,
    \[\frac{d}{dx}[\ln{(1-x)}]=-1\cdot\frac{1}{1-x}=\frac{-1}{1-x}.\]

    So, the base case holds.

    By the inductive hypothesis, we assume that the formula holds for $n=k$.

    For the inductive step, we will find $\frac{d^{k+1}}{dx^{k+1}}[\ln{(1-x)}]$ by differentiating $\frac{d}{dx}[\ln{(1-x)}]$.
    \begin{align*}
        & \frac{d}{dx} \left[ (k-1)!{(-1)}^k{(1-x)}^{-k} \right] \\
        =& (k-1)!{(-1)}^k\frac{d}{dx} \left[ {(1-x)}^{-k} \right] \\
        =& (k-1)!{(-1)}^k\cdot\left( (-k){(1-x)}^{-k-1} \right) \\
        =& k(k-1)!{(-1)}^{k+1}{(1-x)}^{-(k+1)} \\
        =& \left( (k+1)-1 \right)!{(-1)}^{k+1}{(1-x)}^{-(k+1)}, \\
    \end{align*}

    which is the case when $n=k+1$.

    So, the proposition holds.
    
\end{proof}

\end{document}