\documentclass[../hw3]{subfiles}
\begin{document}
\begin{problem}
Snow that the series \[
	1+\frac{x^3}{2\cdot 3} + \frac{x^6}{2\cdot 3\cdot 5\cdot 6} + \cdots+\frac{x^{3n}}{2\cdot 3\cdot 5\cdot 6\cdots(3n-1)(3n)}
\] converges for all $x$, and that the sum satisfied  $f''(x)=xf(x)$.
\end{problem}
\begin{proof}
	Let $f(x)=\sum_{0}^{\infty} a_n x^{3n}$ where $a_0=1$ and $a_n = {\left( \prod_1^n (3k-1)(3k) \right)}^{-1} $.

	By the ratio test, we have that \[
		\left| \frac{a_{n+1}x^{3(n+1)}}{a_n x^{3n}} \right| = \left| \frac{a_{n+1}}{a_n} \right| |x|^3
		.\]

	Then,\[
		a_{n+1} = {\left( \prod_1^{n+1}(3k-1)(3k) \right) }^{-1} = \frac{a_n}{(3(n+1)-1)(3(n+1))}=\frac{a_n}{(3n+2)(3n+3)}
		.\]

	So, \[
		\lim_{n \to \infty} \left| \frac{a_{n+1}}{a_n} \right| \approx \lim_{n \to \infty} O\left( \frac{1}{9n^2} \right) = 0
		.\]

	Thus, the series converges for all $x$.

	Then we have $f''(x)=\sum_{1}^{\infty} (3n)(3n-1)a_n x^{3n-2}$ and $xf(x) = \sum_{0}^{\infty} a_n x^{3n+1}.$
	We will shift the index of the second series by 1, then we have $\sum_{1}^{\infty} a_{n-1}x^{3n-2}$.

	But, $a_{n-1}=(3n)(3n-1)a_n$.
	So, \[
		f''(x)=\sum_{1}^{\infty} (3n)(3n-1)a_n x^{3n-2} = xf(x)
		.\]
\end{proof}
\end{document}
