\documentclass[../hw3]{subfiles}
\begin{document}
\begin{problem}
Express the following series in terms of  elementary functions and their antiderivatives.
\end{problem}
\begin{enumerate}[label=\alph*)]
	\item $\sum_{1}^{\infty} \frac{nx^n}{(n+1)!}$.

	      \begin{align*}
		      \sum_{0}^{\infty} \frac{x^{n + 1}}{(n+1)!} & = e^x - 1                          \\
		      \sum_{0}^{\infty} \frac{x^n}{(n+1)!}       & = \frac{e^x-1}{x}                  \\
		      \sum_{1}^{\infty} \frac{nx^{n-1}}{(n+1)!}  & = \left( \frac{e^x-1}{x} \right)'  \\
		      \sum_{n=1}^{\infty} \frac{nx^n}{(n+1)!}    & = x\left( \frac{e^x-1}{x} \right)'
		      .\end{align*}

	      Now, \[
		      x\left( \frac{e^x -1}{x} \right)' = x\left( \frac{xe^x -(e^x -1)}{x^2} \right) = \frac{xe^x -e^x +1}{x}
		      .\]

	\item $\sum_{0}^{\infty} \frac{(-1)^n x^{2n+1}}{(2n+1)(2n+2)!}$.

	      \begin{align*}
		      \sum_{0}^{\infty} \frac{(-1)^{n+1}x^{2(n+1)}}{(2(n+1))!} & = \cos{x}-1                                \\
		      \sum_{0}^{\infty} \frac{(-1)^n x^{2n}}{(2n+2)!}          & = \frac{1-\cos{x} }{x^2}                   \\
		      \sum_{0}^{\infty} \frac{(-1)^n x^{2n+1}}{(2n+1)(2n+2)!}  & = \int_{0}^{x} \frac{1-\cos{t} }{t^2} \,dt
		      .\end{align*}

	\item $\sum_{0}^{\infty} \frac{x^n}{(n+1)^2 n!}$.

	      \begin{align*}
		      \sum \frac{x^n}{n!}          & = e^x                                           \\
		      \sum \frac{x^{n+1}}{(n+1)n!} & = \int_{0}^{x} e^t \,dt = e^x-1                 \\
		      \sum \frac{x^n}{(n+1)n!}     & = \frac{e^x -1}{x}                              \\
		      \sum \frac{x^n}{(n+1)^2 n!}  & = \frac{1}{x}\int_{0}^{x} \frac{e^t-1}{t}  \,dt
		      .\end{align*}
\end{enumerate}
\end{document}
