\documentclass[../hw3]{subfiles}
\begin{document}
\begin{problem}
Consider $f(x)=\int_{0}^{x} \arctan{t}  \,dt$.
\end{problem}
\begin{enumerate}[label=\alph*)]
	\item Integrate to evaluate $f$ in terms of elementary functions.

	      By IBP, \[
		      \int_{0}^{x} \arctan{t}  \,dt  = \left[ t\arctan{t}-\frac{1}{2}\log{(1+t^2)}   \right]_0^x = x\arctan{x}-\frac{1}{2}\log{(1+x^2)}
		      .\]

	\item Using the arctangent series, compute the Taylor Series of $f$ and show that it converges when $|x| \le 1$.

	      We have that, \[
		      \sum_{0}^{\infty} \frac{(-1)^n x^{2n+1}}{2n+1} = \arctan{x},\,  \forall |x|<1
		      .\]

	      Then, \[
		      \int_{0}^{x} \arctan{t}  \,dt = \sum_{0}^{\infty} \int_{0}^{x} \frac{(-1)^nt^{n+1}}{2n+1} \,dt = \sum_{0}^{\infty} \frac{(-1)^n x^{2n+2}}{(2n+1)(2n+2)}
		      .\]

	      Note that, for all fixed $|x|\le 1$, this series is of order  $\frac{1}{4n^2}$, which converges.

	\item Conclude that \[
		      1-\frac{1}{2} - \frac{1}{3}  + \frac{1}{4} + \frac{1}{5}  - \frac{1}{6}  - \frac{1}{7}  + \cdots = \frac{\pi}{4} - \frac{1}{2}\log{2}
		      .\]
	      We have that \[
		      \int_{0}^{1} \arctan{t}  \,dt = \arctan{1}-\frac{1}{2}\log{(1+1^2)}  = \frac{\pi}{4}-\frac{1}{2}\log{2}
		      .\] .

	      We also have that \[
		      \sum_{0}^{\infty} \frac{(-1)^n}{(2n+1)(2n+2)} = \sum_{0}^{\infty} (-1)^n \left( \frac{1}{2n+1} - \frac{1}{2n+2}\right) = 1-\frac{1}{2} - \frac{1}{3}  + \frac{1}{4} + \frac{1}{5}  - \frac{1}{6}  - \frac{1}{7}  + \cdots
		      .\]
	      Thus, the statement holds.
\end{enumerate}
\end{document}
