\documentclass[../m134a-hw2.tex]{subfiles}

\begin{document}

\subsection*{61e}
Calculate \[\lim\limits_{h \to 0} \frac{f(x+h) - f(x)}{h}\]
for $f(x)=x^n : n \in \mathbb{Z}^+$ %where $n$ is an arbitrary positive integer.
%Make a guess and confirm by induction.

% \begin{proposition}
%     The limit of a sum of functions is equal to the sum of the limits.
% \end{proposition}

% \begin{proposition}
%     For a function $f$ and $\alpha \in \mathbb{R}$, $\lim\limits_{x \to c} \alpha f(x) = \alpha\lim\limits_{x \to c} f(x)$
% \end{proposition}

% \begin{proposition}
%     The limit of a product of functions is equal to the product of the limits.
% \end{proposition}

\begin{proposition}
    $\lim\limits_{h \to 0} \frac{f(x+h) - f(x)}{h} = nx^{n-1}$.
\end{proposition}

\begin{proof}
    Proof by induction.

    For the base case $n=1$, $f(x)=x$.
    \[\lim\limits_{h \to 0} \frac{f(x+h) - f(x)}{h} = 1x^{1-1} = 1x^0 = 1.\]

    So, the statement holds for the base case.

    Next, we assume that the statement holds for $n = k$ such that $f(x) = x^k$ by the inductive hypothesis.
    \[\lim\limits_{h\to0} \frac{{(x+h)}^k-x^k}{h} = kx^{k-1}.\]

    Then, for the inductive step, when $n = k+1$,
    \begin{align*}
        \lim\limits_{h \to 0} \frac{{(x+h)}^{k+1}-x^{k+1}}{h} &= \lim\limits_{h \to 0} \frac{(x+h){(x+h)}^k-x^{k+1}}{h} \\
        &= \lim\limits_{h \to 0} \frac{x{(x+h)}^k+h{(x+h)}^k-x^{k+1}}{h} \\
        &= \lim\limits_{h \to 0} \frac{x{(x+h)}^k-x^{k+1}}{h} + \lim\limits_{h \to 0} \frac{h{(x+h)}^k}{h} \\
        &= \lim\limits_{h \to 0} x \frac{{(x+h)}^k-x^k}{h} + \lim\limits_{h \to 0} {(x+h)}^k \\
    \end{align*}
    If $g$ is a polynomial in $h$, then $x$ is constant. So, $\lim\limits_{h \to 0} g(x + h) = g(x)$.
    
    So, with $g(x) = x^k$, then $\lim\limits_{h \to 0} {(x+h)}^k = \lim\limits_{h \to 0} g(x+h) = g(x) = x^k$.

    Additionally, we recognize that the first quantity is equal to $x \cdot kx^{k-1}$ by the induction hypothesis and the fact that $x$ is constant when taking the limit with respect to $h$.
    \begin{align*}
        \lim\limits_{h \to 0} x \frac{{(x+h)}^k-x^k}{h} + \lim\limits_{h \to 0} {(x+h)}^k &= x \cdot kx^{k-1} + x^k \\
        &= kx^k + k^k \\
        &= (k+1)x^k \\
        &= (k+1)x^{(k+1)-1} \\
    \end{align*}
    Which is the statement when $n = k+1$. Therefore, by induction, the statement holds for all $n \in \mathbb{Z}^+$.
    
\end{proof}

\end{document}