\documentclass[../hw6]{subfiles}

\begin{document}

\subsection*{21.30}

Find the general solution to $y'''-2y''+y'=2e^x+2x$ with the initial conditions $y(0)=y'(0)=y''(0)=0$.

Then, via the characteristic equation, the homogeneous solution is
\[y_h=c_1e^x+c_2xe^x+c_3\]

Since the characteristic equation contains a root of degree two and the non-homogeneous equation contains an $e^x$ term, the form of the particular solution is given by two degrees above the highest degree present in the homogeneous solution,
\[y_p=A+Bx+Cx^2+Ex^2e^x+Fx^3e^x.\]

Then, we also have
\[u_p'=B+2Cx+(Ex^2+2Ex)e^x+(Fx^3+3Ex^2)e^x,\]
and
\[u_p''=2C+(Ex^2+4Ex+2x)e^x+(Fx^3+6Fx^2+6Fx)e^x.\]

Then, 
\begin{align*}
u_p''-2u_p'+u_p&=2e^x+2x\\
A+Bx+Cx^2-2B-4Cx+2C+2Ee^x+5Fxe^x&=2e^x+2x\\
(A-2B+2C)+(B-4C)x+Cx^2+2Ee^x+5Fxe^x&=2e^x+2x.\\
\end{align*}

The system of equations yields\footnote{Did not have time to finish typing up the solution.}\dots

The initial conditions reveal the final solution\footnote{Same as above.}\dots

So \[y=x^2+4x+4+(x^2-4)e^x.\]

\end{document}
