\documentclass[../hw9]{subfiles}

\begin{document}

Since ${||\mathbf{a}||}^2=\mathbf{a}\cdot\mathbf{a}$, then
\begin{align*}
    &{||\mathbf{a}+\mathbf{b}||}^2+{||\mathbf{a}-\mathbf{b}||}^2\\
    =&(\mathbf{a}+\mathbf{b})\cdot(\mathbf{a}+\mathbf{b})+(\mathbf{a}-\mathbf{b})\cdot(\mathbf{a}-\mathbf{b})\\
    =&\mathbf{a}\cdot\mathbf{a}+2(\mathbf{a}\cdot\mathbf{b})+\mathbf{b}\cdot\mathbf{b}+\mathbf{a}\cdot\mathbf{a}-2(\mathbf{a}\cdot\mathbf{b})+\mathbf{b}\cdot\mathbf{b}\\
    =&2(\mathbf{a}\cdot\mathbf{a})+2(\mathbf{b}\cdot\mathbf{b})\\
    =&2({||\mathbf{a}||}^2+{||\mathbf{b}||}^2).
\end{align*}

\end{document}
